compcertxo/Composition.v
@@ -1,0 +1,48 @@
+Require Import CatComp.
+Require Import Linking.
+
+Definition layer_combine {K} (M: Clight.program) (L: layer K) sk :=
+  (* let L' := CatComp.semantics (semantics1 M @ K) (closed_sem_conv L (li_c @ K)) sk *)
+  (* in closed_sem_conv L' li_null. *)
+  layer_comp (semantics1 M @ K) L sk.
+Record prog_ksim {K1 K2: Type} :=
+  mk_prog_ksim {
+      L1: layer K1;
+      L2: layer K2;
+      M: Clight.program;
+      R: krel K1 K2;
+      sk: AST.program unit unit;
+
+      layer_sim: forward_simulation 1 (kcc_ext R) L1 (layer_combine M L2 sk);
+      link_sk: link (skel (semantics1 M)) (skel L2) = Some sk;
+    }.
+
+Section PROG_SIM.
+  Context {K1 K2} (pksim: @prog_ksim K1 K2).
+  Program Definition prog_sim_coercion: @Ksim.ksim K1 K2 :=
+    {|Ksim.L1 := L1 pksim;
+      Ksim.L2 := layer_combine (M pksim) (L2 pksim) (sk pksim);
+      Ksim.R := R pksim; |}.
+  Next Obligation.
+    exact (layer_sim pksim).
+  Qed.
+End PROG_SIM.
+Coercion prog_sim_coercion : prog_ksim >-> Ksim.ksim.
+
+Section VCOMP.
+
+  Context {K1 K2 K3 L1 L2 L3} {M N: Clight.program}
+          {R: krel K1 K2} {S: krel K2 K3} {sk1 sk2}
+          (Hsk1: link (skel L2) (skel (semantics1 M)) = Some sk1)
+          (Hsk2: link (skel L3) (skel (semantics1 N)) = Some sk2)
+          (HL1: forward_simulation 1 (kcc_ext R) L1 (layer_combine M L2 sk1))
+          (HL2: forward_simulation 1 (kcc_ext S) L2 (layer_combine N L3 sk2)).
+  Context (p: Clight.program) (Hlk: link M N = Some p).
+
+  Theorem layer_vcomp:
+    forward_simulation 1 (kcc_ext (krel_comp R S)) L1 (layer_combine p L3 sk2).
+  Proof.
+
+End VCOMP.
+
+Require Import FlatComp.
